Agile implementation, using the latest features

code/hash/Hacl.SHA2Again.fst
@@ -7,7 +7,7 @@ module S = FStar.Seq
 module B = LowStar.Buffer
 module HS = FStar.HyperStack
 module ST = FStar.HyperStack.ST
-module D = FStar.Tactics.Derived
+module T = FStar.Tactics
 
 friend Spec.SHA2Again
 
@@ -26,10 +26,6 @@ let hashes a s l =
   Spec.hashes a s l
 
 let alloca a () =
-  C.h224_reveal ();
-  C.h256_reveal ();
-  C.h384_reveal ();
-  C.h512_reveal ();
   [@ inline_let ]
   let l: list (word a) = Spec.(match a with
     | SHA2_224 -> C.h224_l
@@ -38,18 +34,38 @@ let alloca a () =
     | SHA2_512 -> C.h512_l) in
   B.alloca_of_list l
 
-let alloca_224 = D.specialize (alloca Spec.SHA2_224) []
-let alloca_256 = D.specialize (alloca Spec.SHA2_256) []
-let alloca_384 = D.specialize (alloca Spec.SHA2_384) []
-let alloca_512 = D.specialize (alloca Spec.SHA2_512) []
+let alloca_224: alloca_t Spec.SHA2_224 =
+  T.(synth_by_tactic (specialize (alloca Spec.SHA2_224) [`%alloca]))
+let alloca_256: alloca_t Spec.SHA2_256 =
+  T.(synth_by_tactic (specialize (alloca Spec.SHA2_256) [`%alloca]))
+let alloca_384: alloca_t Spec.SHA2_384 =
+  T.(synth_by_tactic (specialize (alloca Spec.SHA2_384) [`%alloca]))
+let alloca_512: alloca_t Spec.SHA2_512 =
+  T.(synth_by_tactic (specialize (alloca Spec.SHA2_512) [`%alloca]))
+
+let assign_224: B.assign_list_t C.h224_l =
+  T.(synth_by_tactic (specialize (B.assign_list C.h224_l) [`%B.assign_list]))
+let assign_256: B.assign_list_t C.h256_l =
+  T.(synth_by_tactic (specialize (B.assign_list C.h256_l) [`%B.assign_list]))
+let assign_384: B.assign_list_t C.h384_l =
+  T.(synth_by_tactic (specialize (B.assign_list C.h384_l) [`%B.assign_list]))
+let assign_512: B.assign_list_t C.h512_l =
+  T.(synth_by_tactic (specialize (B.assign_list C.h512_l) [`%B.assign_list]))
 
 let init a s =
   let open Spec in
   match a with
-  | SHA2_224 -> C.h224_reveal (); B.blit h224 0ul s 0ul 8ul
-  | _ -> admit ()
+  | SHA2_224 -> assign_224 s
+  | SHA2_256 -> assign_256 s
+  | SHA2_384 -> assign_384 s
+  | SHA2_512 -> assign_512 s
 
-let init_224 = D.specialize (init Spec.SHA2_224) []
-let init_256 = D.specialize (init Spec.SHA2_256) []
-let init_384 = D.specialize (init Spec.SHA2_384) []
-let init_512 = D.specialize (init Spec.SHA2_512) []
+let init_224: init_t Spec.SHA2_224 =
+  T.(synth_by_tactic (specialize (init Spec.SHA2_224) [`%init]))
+let init_256: init_t Spec.SHA2_256 =
+  T.(synth_by_tactic (specialize (init Spec.SHA2_256) [`%init]))
+let init_384: init_t Spec.SHA2_384 =
+  T.(synth_by_tactic (specialize (init Spec.SHA2_384) [`%init]))
+let init_512: init_t Spec.SHA2_512 =
+  T.(synth_by_tactic (specialize (init Spec.SHA2_512) [`%init]))
+
